theories/Dot/experiments.v
@@ -233,9 +233,9 @@ Section Sec.
   Lemma T_self_sem_psingleton Γ p T i :
     (Γ ⊨p p : T , i) -∗
     (* (Γ ⊨p p : sem_psingleton p , i) *)
-    (□∀ vs, ⟦Γ⟧* vs →
-      ▷^i path_wp (p.|[to_subst vs])
-      (λ v, sem_psingleton p (to_subst vs) v)).
+    (□∀ ρ, ⟦Γ⟧* ρ →
+      ▷^i path_wp (p.|[ρ])
+      (λ v, sem_psingleton p ρ v)).
   Proof.
     iIntros "#Hp !>" (vs) "#Hg".
     iSpecialize ("Hp" with "Hg"); iNext i.
