theories/ty_interp_subst_lemmas.v
@@ -4,8 +4,8 @@ From iris.proofmode Require Import tactics.
 Module Type TyInterpLemmas (Import VS : VlSortsFullSig) (Import LWP : LiftWp VS).
 
 Class TyInterpLemmas ty Σ `{sort_ty : Sort ty} `{!TyInterp ty Σ} := {
-  interp_subst_compose_ind T sb1 sb2 v:
-    ⟦ T.|[sb1] ⟧ sb2 v ⊣⊢ ⟦ T ⟧ (sb1 >> sb2) v;
+  interp_subst_compose_ind T ρ1 ρ2 v:
+    ⟦ T.|[ρ1] ⟧ ρ2 v ⊣⊢ ⟦ T ⟧ (ρ1 >> ρ2) v;
 }.
 
 (** * Lemmas about the logical relation itself. *)
@@ -13,59 +13,37 @@ Section logrel_binding_lemmas.
   Context `{Htil : TyInterpLemmas ty Σ}.
 
   Implicit Types
-          (L T U: ty) (v: vl) (e: tm)
-          (ρ : vls).
+          (L T U: ty) (v: vl) (e: tm) (ρ : env).
 
-  Lemma interp_subst_compose T sb1 sb2 sb3:
-    sb1 >> sb2 = sb3 → ⟦ T.|[sb1] ⟧ sb2 ≡ ⟦ T ⟧ sb3.
+  Lemma interp_subst_compose T ρ1 ρ2 ρ3:
+    ρ1 >> ρ2 = ρ3 → ⟦ T.|[ρ1] ⟧ ρ2 ≡ ⟦ T ⟧ ρ3.
   Proof. move=> <- v. exact: interp_subst_compose_ind. Qed.
 
-  Lemma interp_weaken_one v τ ρ:
-     ⟦ τ.|[ren (+1)] ⟧ (v .: to_subst ρ) ≡ ⟦ τ ⟧ (to_subst ρ).
-  Proof. apply interp_subst_compose, (to_subst_weaken [] [v]). Qed.
+  Lemma interp_weaken_one τ ρ:
+     ⟦ τ.|[ren (+1)] ⟧ ρ ≡ ⟦ τ ⟧ ((+1) >>> ρ).
+  Proof. apply interp_subst_compose. autosubst. Qed.
 
-  Lemma interp_subst ρ τ v1 v2 :
-    ⟦ τ.|[v1.[ren (+length ρ)]/] ⟧ (to_subst ρ) v2 ≡
-    ⟦ τ ⟧ (v1 .: to_subst ρ) v2.
-  Proof. apply interp_subst_compose, (to_subst_up []). Qed.
+  Lemma interp_subst_one T v w ρ:
+    ⟦ T.|[v/] ⟧ ρ w ≡ ⟦ T ⟧ (v.[ρ] .: ρ) w.
+  Proof. apply interp_subst_compose. autosubst. Qed.
 
-  Lemma interp_subst_ids T sb1 : ⟦ T ⟧ sb1 ≡ ⟦ T.|[sb1] ⟧ ids.
+  Lemma interp_subst_ids T ρ : ⟦ T ⟧ ρ ≡ ⟦ T.|[ρ] ⟧ ids.
   Proof. symmetry. apply interp_subst_compose. autosubst. Qed.
 
-  Lemma interp_nclosed_proper {T n sb1 sb2}:
-    nclosed T n → eq_n_s sb1 sb2 n → ⟦ T.|[sb1] ⟧ ≡ ⟦ T.|[sb2] ⟧.
-  Proof. intros HclT Heqs. f_equiv. apply HclT, Heqs. Qed.
-
-  Lemma interp_closed {T n sb1 sb2}:
-    nclosed T n → eq_n_s sb1 sb2 n → ⟦ T ⟧ sb1 ≡ ⟦ T ⟧ sb2.
-  Proof.
-    move => Hcl Heqs.
-    rewrite (interp_subst_ids T sb1) (interp_subst_ids T sb2).
-    exact: interp_nclosed_proper.
-  Qed.
-
-  Lemma interp_subst_commute_gen T {σ sb v}:
-    ⟦ T.|[to_subst σ] ⟧ sb v ≡ ⟦ T ⟧ (to_subst σ >> sb) v.
-  Proof. exact: interp_subst_compose. Qed.
-
-  (*
+  (**
     We have, unconditionally, that
-    ⟦ T.|[to_subst σ] ⟧ sb = ⟦ T ⟧ (to_subst σ >> sb).
+    ⟦ T.|[to_subst σ] ⟧ ρ = ⟦ T ⟧ (to_subst σ >> ρ).
 
-    But [to_subst σ >> sb] and [to_subst σ.|[sb]] are only equal for
+    But [to_subst σ >> ρ] and [to_subst σ.|[ρ]] are only equal for
     [length σ] entries.
   *)
-  Lemma interp_subst_commute T σ sb v:
+  Lemma interp_subst_commute T σ ρ v:
     nclosed T (length σ) →
-    ⟦ T.|[to_subst σ] ⟧ sb v ≡ ⟦ T ⟧ (to_subst σ.|[sb]) v.
+    ⟦ T.|[∞ σ] ⟧ ρ v ≡ ⟦ T ⟧ (∞ σ.|[ρ]) v.
   Proof.
-    rewrite interp_subst_commute_gen => HclT. symmetry.
-    apply (interp_closed HclT).
-    apply to_subst_compose.
+    move => HclT. rewrite interp_subst_compose_ind.
+    rewrite (interp_subst_ids T (∞ _) v) (interp_subst_ids T (_ >> _) v).
+    rewrite (subst_compose _ _ HclT) //. f_equiv; autosubst.
   Qed.
-
-  Lemma interp_subst_closed T v w ρ:
-    ⟦ T.|[v/] ⟧ (to_subst ρ) w ≡ ⟦ T ⟧ (v.[to_subst ρ] .: to_subst ρ) w.
-  Proof. apply interp_subst_compose. autosubst. Qed.
 End logrel_binding_lemmas.
 End TyInterpLemmas.
